new/code/github_com/goose_lang/goose/model/channel.v
@@ -20,7 +20,7 @@ End offerState.
 
 Class offerState_Assumptions {ext : ffi_syntax} `{!GoGlobalContext} `{!GoLocalContext} `{!GoSemanticsFunctions} : Prop :=
 {
-  #[global] offerState_zero_val  :: go.GoZeroValEq offerState offerState.t;
+  #[global] offerState_zero_val  :: go.TypeRepr offerState offerState.t;
   #[global] offerState_underlying :: go.Underlying (offerState) (offerStateⁱᵐᵖˡ);
 }.
 
@@ -414,7 +414,7 @@ End Channel.
 
 Class Channel_Assumptions {ext : ffi_syntax} `{!GoGlobalContext} `{!GoLocalContext} `{!GoSemanticsFunctions} : Prop :=
 {
-  #[global] Channel_zero_val T T' `{!ZeroVal T'} `{!go.GoZeroValEq T T'} :: go.GoZeroValEq (Channel T) (Channel.t T');
+  #[global] Channel_zero_val T T' `{!ZeroVal T'} `{!go.TypeRepr T T'} :: go.TypeRepr (Channel T) (Channel.t T');
   #[global] Channel_underlying T :: go.Underlying (Channel T) (Channelⁱᵐᵖˡ T);
   #[global] Channel_get_cap T T' (x : Channel.t T') :: go.IsGoStepPureDet (StructFieldGet (Channel T) "cap") #x #x.(Channel.cap);
   #[global] Channel_set_cap T T' (x : Channel.t T') y :: go.IsGoStepPureDet (StructFieldSet (Channel T) "cap") (#x, #y) #(x <|Channel.cap := y|>);
@@ -467,7 +467,7 @@ End SelectDir.
 
 Class SelectDir_Assumptions {ext : ffi_syntax} `{!GoGlobalContext} `{!GoLocalContext} `{!GoSemanticsFunctions} : Prop :=
 {
-  #[global] SelectDir_zero_val  :: go.GoZeroValEq SelectDir SelectDir.t;
+  #[global] SelectDir_zero_val  :: go.TypeRepr SelectDir SelectDir.t;
   #[global] SelectDir_underlying :: go.Underlying (SelectDir) (SelectDirⁱᵐᵖˡ);
 }.
 
